Phi_Semantics/PhiSem_Mem_C_Array.thy
@@ -3,7 +3,7 @@ theory PhiSem_Mem_C_Array
 begin
 
 debt_axiomatization
-    memobj_size_arr: \<open>MemObj_Size (array N T) = N * MemObj_Size T\<close>
+    memobj_size_arr: \<open>MemObj_Size (\<a>\<r>\<r>\<a>\<y>[N] T) = N * MemObj_Size T\<close>
 and Map_of_Val_arr: \<open>Map_of_Val (V_array.mk vs) = nnode (map Map_of_Val vs)\<close>
 
 
