Phi_Semantics/PhiSem_Mem_C_MI.thy
@@ -5,26 +5,26 @@ begin
 proc op_allocate_mem_N:
   input \<open>n \<Ztypecolon> \<v>\<a>\<l> \<nat>(size_t)\<close>
   requires \<open>Semantic_Zero_Val TY T z\<close>
-  output \<open>replicate n z \<Ztypecolon> \<m>\<e>\<m>[addr] (\<m>\<e>\<m>-\<c>\<o>\<e>\<r>\<c>\<e> (Array n T))\<heavy_comma> addr \<Ztypecolon> \<v>\<a>\<l> Ptr (array n TY) \<s>\<u>\<b>\<j> addr. memaddr.index addr = 0\<close>
+  output \<open>replicate n z \<Ztypecolon> \<m>\<e>\<m>[addr] (\<m>\<e>\<m>-\<c>\<o>\<e>\<r>\<c>\<e> (Array n T))\<heavy_comma> addr \<Ztypecolon> \<v>\<a>\<l> Ptr (\<a>\<r>\<r>\<a>\<y>[n] TY) \<s>\<u>\<b>\<j> addr. memaddr.index addr = 0\<close>
   including Semantic_Zero_Val_EIF_brute
 \<medium_left_bracket>
   note list_all2_conv_all_nth[simp] ;;
 
   semantic_local_value($n) \<open>\<i>\<n>\<t>(size_t)\<close>
   semantic_assert \<open>Zero TY \<noteq> None\<close>
-  apply_rule FIC.aggregate_mem.allocate_rule[where TY=\<open>array n TY\<close>
+  apply_rule FIC.aggregate_mem.allocate_rule[where TY=\<open>\<a>\<r>\<r>\<a>\<y>[n] TY\<close>
                                                and v=\<open>V_array.mk (replicate (snd (V_int.dest (\<phi>arg.dest \<a>\<r>\<g>1))) (the (Zero TY)))\<close>]
 
-  semantic_assumption \<open>type_storable_in_mem (array (snd (V_int.dest (\<phi>arg.dest \<a>\<r>\<g>1))) TY)\<close>
+  semantic_assumption \<open>type_storable_in_mem (\<a>\<r>\<r>\<a>\<y>[snd (V_int.dest (\<phi>arg.dest \<a>\<r>\<g>1))] TY)\<close>
 
   \<open>replicate n z \<Ztypecolon> MAKE (\<m>\<e>\<m>[memaddr blk 0] (MAKE (\<m>\<e>\<m>-\<c>\<o>\<e>\<r>\<c>\<e> (Array n T))))\<close>
 
   have t1: \<open>valid_logaddr (memaddr blk [])\<close>
     unfolding valid_logaddr_def Valid_MemBlk_def
-    using \<open>memblk.layout blk = array n TY\<close>
-    by (cases blk; clarsimp simp: \<open>type_storable_in_mem (array n TY)\<close>) ;;
+    using \<open>memblk.layout blk = \<a>\<r>\<r>\<a>\<y>[n] TY\<close>
+    by (cases blk; clarsimp simp: \<open>type_storable_in_mem (\<a>\<r>\<r>\<a>\<y>[n] TY)\<close>) ;;
   
-  semantic_return \<open>V_pointer.mk (memaddr (\<phi>arg.dest \<v>2) 0) \<Turnstile> (memaddr blk 0 \<Ztypecolon> Ptr (array n TY))\<close>
+  semantic_return \<open>V_pointer.mk (memaddr (\<phi>arg.dest \<v>2) 0) \<Turnstile> (memaddr blk 0 \<Ztypecolon> Ptr (\<a>\<r>\<r>\<a>\<y>[n] TY))\<close>
 
 \<medium_right_bracket> .
 
