Phi_Semantics/PhiSem_Mem_Pointer.thy
@@ -4,7 +4,7 @@ theory PhiSem_Mem_Pointer
       "\<tribullet>" :: quasi_command
   abbrevs "+_a" = "+\<^sub>a"
       and "\<tribullet>_a"  = "\<tribullet>\<^sub>a"
-      and "<Ptr>" = "\<bbbP>\<t>\<r>"
+      and "<Ptr>" = "\<Pp>\<t>\<r>"
       and "<ptr>" = "\<p>\<t>\<r>"
 begin
 
@@ -574,7 +574,7 @@ lemma RawPointer_eqcmp[\<phi>reason 1200]:
 
 subsubsection \<open>Logical Pointer\<close>
 
-\<phi>type_def Ptr :: "TY \<Rightarrow> (VAL, logaddr) \<phi>" ("\<bbbP>\<t>\<r> _" [999] 998)
+\<phi>type_def Ptr :: "TY \<Rightarrow> (VAL, logaddr) \<phi>" ("\<Pp>\<t>\<r> _" [999] 998)
   where \<open>x \<Ztypecolon> Ptr TY \<equiv> V_pointer.mk (logaddr_to_raw x) \<Ztypecolon> Itself \<s>\<u>\<b>\<j> valid_logaddr x \<and> logaddr_type x = TY\<close>
   deriving Basic
        and \<open>Object_Equiv (Ptr TY) (=)\<close>
